WIP (helper lemmas now done -- except for one strange admit)

examples/invariants/DY.Example.Invariants.Uniqueness.fst
@@ -128,6 +128,26 @@ let rec zero_to_sid_mem (bound:state_id) (x :state_id{x.the_id <= bound.the_id})
         zero_to_sid_mem ({the_id = bound.the_id -1}) x
     end
 
+let rec zero_to_sid_mems (bound:state_id) (sid:state_id) :
+  Lemma 
+  (requires
+    sid `List.mem` (zero_to_sid bound)
+  )
+  ( ensures
+  sid.the_id <= bound.the_id
+  )
+  (decreases bound.the_id)
+  = if bound.the_id = 0
+    then ()
+    else (
+      if sid = bound
+      then ()
+      else (
+     FStar.List.Tot.Properties.append_mem_forall (zero_to_sid {the_id = bound.the_id - 1}) [bound];
+     zero_to_sid_mems ({the_id =bound.the_id - 1}) sid
+     )
+  )
+
 let no_set_state_entry_for_p (p:principal) (tr:trace) =
   forall sid. no_set_state_entry_for p sid tr
 
@@ -185,22 +205,6 @@ let get_full_state_same (p:principal) (tr1:trace) (tr2:trace):
     (get_session_indexed tr2 p) 
     (zero_to_sid (compute_new_session_id p tr1))
   
-
-
-let get_full_state_on_growing_traces (p:principal) (tr1 tr2:trace) (sid:state_id):
-  Lemma 
-  (requires
-    tr1 <$ tr2
-    /\ Some? (get_full_state p tr1)
-  )
-  (ensures
-    Some? (get_full_state p tr2) /\
-    sid `List.mem` (List.map fst (Some?.v (get_full_state p tr1)))
-    ==>
-    sid `List.mem` (List.map fst (Some?.v (get_full_state p tr2)))
-  )
-  = admit()
-
 let rec mem_choose (#a #b:eqtype) (f: a -> option b) (xs : list a) (x:a):
   Lemma
   (requires 
@@ -214,6 +218,206 @@ let rec mem_choose (#a #b:eqtype) (f: a -> option b) (xs : list a) (x:a):
       if hd = x
       then ()
       else mem_choose f tl x 
+
+
+let rec mem_choose_elim (#a #b:eqtype) (f: a -> option b) (xs : list a) (y : b)
+  : Lemma
+  (ensures (
+    y `List.mem` (List.choose f xs) ==> 
+    (exists x. x `List.mem` xs /\ Some? (f x) /\ Some?.v (f x) = y)
+    )
+  )
+  =match xs with
+  | [] -> ()
+  | hd :: tl -> mem_choose_elim f tl y
+
+let rec compute_new_session_id_grows (p:principal) (tr1 tr2:trace):
+  Lemma 
+  (requires tr1 <$ tr2
+  )
+  (ensures
+    (compute_new_session_id p tr1).the_id <= (compute_new_session_id p tr2).the_id
+  )
+  = reveal_opaque (`%grows) grows; 
+    norm_spec [zeta; delta_only [`%prefix]] (prefix);
+    if tr1 = tr2
+    then ()
+    else (
+      match tr2 with
+      | Nil -> ()
+      | Snoc tr2_init tr2_ev -> compute_new_session_id_grows p tr1 tr2_init
+    )
+
+
+val full_state_session_lemma:
+  (tr:trace) -> (p:principal) -> (i:nat) ->
+  Lemma(
+    match get_full_state p tr with 
+      | None -> True
+      | Some full_st -> begin
+          if i >= List.length full_st
+            then True
+            else begin
+              let (sid_i, sess_i) = List.index full_st i in
+              get_session p sid_i tr = Some sess_i
+            end
+      end
+  )
+let full_state_session_lemma tr p i =
+    match get_full_state p tr with 
+      | None -> ()
+      | Some full_st -> begin
+          if i >= List.length full_st
+            then ()
+            else (
+              let (sid_i, sess_i) = List.index full_st i in
+              let next_sid = compute_new_session_id p tr in
+              let sids = zero_to_sid next_sid in
+              let f = get_session_indexed tr p in
+              FStar.List.Tot.Properties.lemma_index_memP full_st i;
+              mem_choose_elim f sids (sid_i, sess_i)
+              )
+      end
+
+let full_state_some_get_session_some (p:principal) (sid:state_id) (tr:trace):
+  Lemma 
+  (requires
+     Some? (get_full_state p tr)
+     /\ sid `List.mem` (List.map fst (Some?.v (get_full_state p tr)))
+  )
+  (ensures
+     Some? (get_session p sid tr)
+  )
+  = let Some full_st = get_full_state p tr in
+    let next_sid = compute_new_session_id p tr in
+    let sids = zero_to_sid next_sid in
+    FStar.List.Tot.Properties.memP_map_elim fst sid full_st;
+    eliminate exists sess. (sid, sess) `List.mem` full_st 
+    returns Some? (get_session p sid tr)
+    with _ .
+      mem_choose_elim (get_session_indexed tr p) sids (sid, sess)
+    
+
+
+let rec get_session_grows (p:principal) (sid:state_id) (tr1 tr2:trace):
+  Lemma
+  ( requires tr1 <$ tr2 /\ Some? (get_session p sid tr1)
+  )
+  (ensures
+    Some? (get_session p sid tr2)
+  )
+ = reveal_opaque (`%grows) grows; 
+   norm_spec [zeta; delta_only [`%prefix]] (prefix);
+   if tr1 = tr2 
+   then ()
+   else (
+     match tr2 with
+     | Nil -> ()
+     | Snoc init _ -> get_session_grows p sid tr1 init
+   )
+
+let last_event_exists (tr:trace):
+  Lemma
+  (requires Snoc? tr
+  )
+  (ensures (
+     let Snoc _ ev = tr in
+     event_exists tr ev
+     )
+  )
+  [SMTPat (Snoc? tr)]
+  = let Snoc _ ev = tr in
+    assert(event_at tr (Trace.length tr - 1) ev)
+
+
+
+let rec get_session_state_was_set (p:principal) (sid:state_id) (tr:trace):
+  Lemma
+  (requires Some? (get_session p sid tr))
+  (ensures exists cont. state_was_set tr p sid cont )
+  = match tr with
+  | Nil -> ()
+  | Snoc init (SetState p' sid' cont') -> (
+         if p' = p && sid' = sid
+         then ()
+         else get_session_state_was_set p sid init
+   )      
+  | Snoc init _ -> 
+        get_session_state_was_set p sid init
+
+let get_session_some_full_state_some (p:principal) (sid:state_id) (tr:trace):
+  Lemma 
+  ( requires Some? (get_session p sid tr)
+  )
+  (ensures Some? (get_full_state p tr)
+  )
+  =
+    get_session_state_was_set p sid tr;
+    eliminate exists cont . state_was_set tr p sid cont
+    returns Some? (get_full_state p tr)
+    with _ .
+        compute_new_session_id_larger_than_id_on_trace p tr sid cont
+
+
+
+let full_state_fst_zero_to_sid (tr:trace) (p:principal):
+  Lemma
+  ( requires Some? (get_full_state p tr)
+  )
+  (ensures (
+    let Some full_st = get_full_state p tr in
+    let next_sid = compute_new_session_id p tr in
+    (List.map fst (full_st)) `List.subset` (zero_to_sid next_sid)
+    )
+  )
+  =
+    let Some full_st = get_full_state p tr in
+    let next_sid = compute_new_session_id p tr in
+  introduce forall sid. sid `List.mem` (List.map fst full_st) ==> sid `List.mem` (zero_to_sid next_sid)
+  with (
+    introduce _ ==> _
+    with _ . (
+      FStar.List.Tot.Properties.memP_map_elim fst sid full_st;
+      eliminate exists sess. (sid, sess) `List.mem` full_st
+      returns _
+      with _ . (
+      mem_choose_elim (get_session_indexed tr p) (zero_to_sid next_sid) (sid,sess)      
+      )
+    )
+  )
+
+let get_full_state_on_growing_traces (p:principal) (tr1 tr2:trace) (sid:state_id):
+  Lemma 
+  (requires
+      tr1 <$ tr2
+    /\ Some? (get_full_state p tr1)
+    /\ sid `List.mem` (List.map fst (Some?.v (get_full_state p tr1)))
+  )
+  (ensures
+    Some? (get_full_state p tr2) /\    
+    sid `List.mem` (List.map fst (Some?.v (get_full_state p tr2)))
+  )
+  = 
+  let Some full_st1 = get_full_state p tr1 in
+ 
+         let new_sid1 = compute_new_session_id p tr1 in
+         let new_sid2 = compute_new_session_id p tr2 in
+         compute_new_session_id_grows p tr1 tr2;
+         let sids1 = zero_to_sid new_sid1 in
+         let sids2 = zero_to_sid new_sid2 in
+         full_state_fst_zero_to_sid tr1 p;
+           zero_to_sid_mems new_sid1 sid;
+           zero_to_sid_mem new_sid2 sid;
+         
+         full_state_some_get_session_some p sid tr1;
+         get_session_grows p sid tr1 tr2;
+         let Some sess2 = get_session p sid tr2 in
+         get_session_some_full_state_some p sid tr2;
+         let Some full_st2 = get_full_state p tr2 in
+         mem_choose (get_session_indexed tr2 p) sids2 sid;
+         FStar.List.Tot.Properties.memP_map_intro fst (sid, sess2) full_st2
+   
+
 
 let rec state_was_set_full_state (tr:trace) (p:principal) (sid:state_id) (cont:bytes):
   Lemma
@@ -257,46 +461,7 @@ let rec state_was_set_full_state (tr:trace) (p:principal) (sid:state_id) (cont:b
      state_was_set_full_state init p sid cont
 
 
-let rec mem_choose_elim (#a #b:eqtype) (f: a -> option b) (xs : list a) (y : b)
-  : Lemma
-  (ensures (
-    y `List.mem` (List.choose f xs) ==> 
-    (exists x. x `List.mem` xs /\ Some? (f x) /\ Some?.v (f x) = y)
-    )
-  )
-  =match xs with
-  | [] -> ()
-  | hd :: tl -> mem_choose_elim f tl y
 
-val full_state_session_lemma:
-  (tr:trace) -> (p:principal) -> (i:nat) ->
-  Lemma(
-    match get_full_state p tr with 
-      | None -> True
-      | Some full_st -> begin
-          if i >= List.length full_st
-            then True
-            else begin
-              let (sid_i, sess_i) = List.index full_st i in
-              get_session p sid_i tr = Some sess_i
-            end
-      end
-  )
-let full_state_session_lemma tr p i =
-    match get_full_state p tr with 
-      | None -> ()
-      | Some full_st -> begin
-          if i >= List.length full_st
-            then ()
-            else (
-              let (sid_i, sess_i) = List.index full_st i in
-              let next_sid = compute_new_session_id p tr in
-              let sids = zero_to_sid next_sid in
-              let f = get_session_indexed tr p in
-              FStar.List.Tot.Properties.lemma_index_memP full_st i;
-              mem_choose_elim f sids (sid_i, sess_i)
-              )
-      end
 
 val parse_full_state_lemma :
   (tr: trace) -> p:principal -> (i:nat) ->
